Refactored the appears_in_tree prop, and changed a ton of proofs to work with it.

code/InductiveDataTypes.v
@@ -19,14 +19,14 @@ Inductive appears_in_kvl {X:Type} (sk: nat) : list (nat * X) -> Prop :=
   | ai_later : forall k v l, appears_in_kvl sk l -> appears_in_kvl sk ((k, v)::l).
   
 Inductive appears_in_tree {X:Type} {b: nat} (sk: nat) : bplustree b X -> Prop :=
-  | ait_leaf       : forall l,       appears_in_kvl sk l -> appears_in_tree sk (bptLeaf b X l)
-  | ait_node_one   : forall k v,     appears_in_tree sk v -> k <= sk ->
-                                     appears_in_tree sk (bptNode b X [(k, v)])
+  | ait_leaf          : forall l,       appears_in_kvl sk l -> appears_in_tree sk (bptLeaf b X l)
+  | ait_node_last : forall k1 k2 v1 v2, appears_in_tree sk v2 -> k2 <= sk ->
+                                     appears_in_tree sk (bptNode b X [(k1, v1), (k2, v2)])
   | ait_node_here  : forall k1 k2 v1 v2 l, 
                                      appears_in_tree sk v1 -> k1 <= sk /\ sk < k2 ->
                                      appears_in_tree sk (bptNode b X ((k1, v1)::(k2, v2)::l))
-  | ait_node_later : forall x k v l, appears_in_tree sk (bptNode b X ((k, v)::l)) -> k <= sk ->
-                                     appears_in_tree sk (bptNode b X (x::(k, v)::l)).
+  | ait_node_later : forall x k1 k2 v1 v2 l, appears_in_tree sk (bptNode b X ((k1, v1)::(k2, v2)::l)) -> k1 <= sk ->
+                                     appears_in_tree sk (bptNode b X (x::(k1, v1)::(k2, v2)::l)).
   
   
 Inductive kvl_sorted {X: Type}: list (nat * X) -> Prop :=
